Proved Goedel's beta lemma

theories/Semantics/IMP/Axiomatic.v
@@ -50,7 +50,7 @@ Fixpoint aexp_to_eaexp (a : AExp L) : EAExp L V :=
   | Mul a1 a2 => EMul (aexp_to_eaexp a1)  (aexp_to_eaexp a2)
   end.
 
-Fixpoint aloc_vars (a : EAExp L V) : Ensemble L :=
+Fixpoint aloc_vars (a : EAExp L V) : listset L :=
   match a with
   | EAVal z => ∅
   | EVar x => {[x]}
@@ -60,7 +60,7 @@ Fixpoint aloc_vars (a : EAExp L V) : Ensemble L :=
   | EMul a1 a2 => aloc_vars a1 ∪ aloc_vars a2
   end.
 
-Fixpoint alog_vars (a : EAExp L V) : Ensemble V :=
+Fixpoint alog_vars (a : EAExp L V) : listset V :=
   match a with
   | EAVal z => ∅
   | EVar x => ∅
@@ -70,10 +70,13 @@ Fixpoint alog_vars (a : EAExp L V) : Ensemble V :=
   | EMul a1 a2 => alog_vars a1 ∪ alog_vars a2
   end.
 
-#[local] Coercion aexp_to_eaexp : AExp >-> EAExp.
+Global Coercion aexp_to_eaexp : AExp >-> EAExp.
 
-Definition eimpl (b1 b2: EBExp L V) : EBExp L V :=
+Definition eb_impl (b1 b2: EBExp L V) : EBExp L V :=
   EOr (ENot b1) b2.
+
+Definition eb_exists (x : V) (b : EBExp L V) : EBExp L V :=
+    ENot (Forall x (ENot b)).
 
 Fixpoint bexp_to_ebexp (b : BExp L) : EBExp L V :=
   match b with
@@ -85,7 +88,7 @@ Fixpoint bexp_to_ebexp (b : BExp L) : EBExp L V :=
   | Or b1 b2 => EOr (bexp_to_ebexp b1) (bexp_to_ebexp b2)
   end.
 
-Fixpoint bloc_vars (b : EBExp L V) : Ensemble L :=
+Fixpoint bloc_vars (b : EBExp L V) : listset L :=
   match b with
   | EBVal t => ∅
   | EAEq a1 a2 => aloc_vars a1 ∪ aloc_vars a2
@@ -96,7 +99,7 @@ Fixpoint bloc_vars (b : EBExp L V) : Ensemble L :=
   | Forall x b => bloc_vars b
   end.
 
-Fixpoint blog_vars (b : EBExp L V) : Ensemble V :=
+Fixpoint blog_vars (b : EBExp L V) : listset V :=
   match b with
   | EBVal t => ∅
   | EAEq a1 a2 => alog_vars a1 ∪ alog_vars a2
@@ -107,7 +110,16 @@ Fixpoint blog_vars (b : EBExp L V) : Ensemble V :=
   | Forall x b => blog_vars b ∖ {[x]}
   end.
 
-#[local] Coercion bexp_to_ebexp : BExp >-> EBExp.
+Global Coercion bexp_to_ebexp : BExp >-> EBExp.
+
+Fixpoint cloc_vars (c : Cmd L) : listset L :=
+match c with
+| Skip => ∅
+| Asgn x a => aloc_vars a ∪ {[x]}
+| Seq c0 c1 => cloc_vars c0 ∪ cloc_vars c1
+| If b c0 c1 => bloc_vars b ∪ cloc_vars c0 ∪ cloc_vars c1
+| While b c => bloc_vars b ∪ cloc_vars c
+end.
 
 Definition substitution (T : Type) : Type := T -> option (AExp L).
 
@@ -181,8 +193,8 @@ Qed.
 
 Lemma asubst_id :
     forall (a : EAExp L V) (slog : substitution V) (sloc : substitution L),
-    aloc_vars a ∩ subst_vars sloc ≡ ∅ ->
-    alog_vars a ∩ subst_vars slog ≡ ∅ ->
+    list_to_set (elements (aloc_vars a)) ∩ subst_vars sloc ≡ ∅ ->
+    list_to_set (elements (alog_vars a)) ∩ subst_vars slog ≡ ∅ ->
     asubst a slog sloc = a.
 Proof.
     intros *; induction a; intros Hloc Hlog.
@@ -206,8 +218,8 @@ Proof.
 Qed.
 
 Lemma bsubst_id : forall (b : EBExp L V) (slog : substitution V) (sloc : substitution L),
-    bloc_vars b ∩ subst_vars sloc ≡ ∅ ->
-    blog_vars b ∩ subst_vars slog ≡ ∅ ->
+    list_to_set (elements (bloc_vars b)) ∩ subst_vars sloc ≡ ∅ ->
+    list_to_set (elements (blog_vars b)) ∩ subst_vars slog ≡ ∅ ->
     bsubst b slog sloc = b.
 Proof.
     induction b; intros slog sloc Hloc Hlog.
@@ -224,8 +236,9 @@ Proof.
       intro x; rewrite elem_of_intersection; intros [Hx [a Ha]].
       unfold fn_update in Ha; case_decide; [done |].
       apply Hlog.
-      rewrite elem_of_intersection, elem_of_difference, elem_of_singleton.
-      by split_and!; [..| eexists].
+      rewrite elem_of_intersection, elem_of_list_to_set, elem_of_elements, elem_of_difference, elem_of_singleton.
+      split_and!; [| done | eexists; done].
+      by apply elem_of_list_to_set, elem_of_elements in Hx.
 Qed.
 
 Definition eaeval (sigma : State L) (I : State V): EAExp L V -> Z :=
@@ -249,6 +262,20 @@ Proof.
     - by cbn; rewrite IHa1, IHa2.
     - by cbn; rewrite IHa1, IHa2.
     - by cbn; rewrite IHa1, IHa2.
+Qed.
+
+Lemma eaeval_update_I :
+    forall (a : EAExp L V) (sigma : State L) (I : State V) (x : V) (z : Z),
+    x ∉ alog_vars a ->
+    eaeval sigma (fn_update I x z) a = eaeval sigma I a.
+Proof.
+    intros *. induction a; cbn; intro Hx.
+    - by unfold fn_update; rewrite decide_False by set_solver.
+    - done.
+    - done.
+    - by rewrite IHa1, IHa2 by set_solver.
+    - by rewrite IHa1, IHa2 by set_solver.
+    - by rewrite IHa1, IHa2 by set_solver.
 Qed.
 
 Lemma top_char X : X ≡ top True <-> I ∈ X.
@@ -328,11 +355,11 @@ Lemma satsi_and_intro : forall (sigma : State L) (I : State V) (b1 b2 : EBExp L 
 Proof. by set_solver. Qed.
 
 Lemma satsi_and_elim_l : forall (sigma : State L) (I : State V) (b1 b2 : EBExp L V),
-    satsi sigma I (EAnd b1 b2) -> satsi sigma I b1. 
+    satsi sigma I (EAnd b1 b2) -> satsi sigma I b1.
 Proof. by set_solver. Qed.
 
 Lemma satsi_and_elim_r : forall (sigma : State L) (I : State V) (b1 b2 : EBExp L V),
-    satsi sigma I (EAnd b1 b2) -> satsi sigma I b2. 
+    satsi sigma I (EAnd b1 b2) -> satsi sigma I b2.
 Proof. by set_solver. Qed.
 
 Lemma satsi_and : forall (sigma : State L) (I : State V) (b1 b2 : EBExp L V),
@@ -351,19 +378,30 @@ Proof.
     by rewrite elem_of_indexed_intersection.
 Qed.
 
-Lemma satsi_mp :  forall (sigma : State L) (I : State V) (b1 b2 : EBExp L V),
-    satsi sigma I (eimpl b1 b2) -> satsi sigma I b1 -> satsi sigma I b2.
+Lemma satsi_exists : forall (sigma : State L) (I : State V) (x : V) (b : EBExp L V),
+    satsi sigma I (eb_exists x b) <-> exists (z : Z), satsi sigma (fn_update I x z) b.
 Proof.
-    intros *; unfold eimpl.
+    intros; unfold eb_exists; rewrite satsi_not, satsi_forall.
+    setoid_rewrite satsi_not.
+    split.
+    - by intro; apply not_all_not_ex.
+    - intros [z Hz] Hall.
+      by eapply Hall.
+Qed.
+
+Lemma satsi_mp :  forall (sigma : State L) (I : State V) (b1 b2 : EBExp L V),
+    satsi sigma I (eb_impl b1 b2) -> satsi sigma I b1 -> satsi sigma I b2.
+Proof.
+    intros *; unfold eb_impl.
     rewrite satsi_or, satsi_not.
     by intros [].
 Qed.
 
 Lemma classical_satsi_impl :  forall (sigma : State L) (I : State V) (b1 b2 : EBExp L V),
-    satsi sigma I (eimpl b1 b2) <-> (satsi sigma I b1 -> satsi sigma I b2).
+    satsi sigma I (eb_impl b1 b2) <-> (satsi sigma I b1 -> satsi sigma I b2).
 Proof.
     split; [by apply satsi_mp |].
-    intros *; unfold eimpl.
+    intros *; unfold eb_impl.
     rewrite satsi_or, satsi_not.
     intros Himpl.
     destruct (classic (satsi sigma I b1)).
@@ -395,6 +433,9 @@ Proof.
       setoid_rewrite IHb1; setoid_rewrite IHb2; cbn.
       by rewrite orb_true_iff.
 Qed.
+
+Definition sati (b : EBExp L V) : Prop :=
+    forall (sigma : State L) (I : State V), satsi sigma I b.
 
 Definition sat (b : EBExp L V) : Prop :=
     forall (sigma : State L) (I : State V), satsi sigma I b.
@@ -444,9 +485,9 @@ Inductive ht_ded : HoareTriple -> Prop :=
     ht_ded (ht (EAnd A b) c A) ->
     ht_ded (ht A (While b c) (EAnd A (ENot b)))
 | ht_cons : forall (A A' B B' : EBExp L V) (c : Cmd L),
-    sat (eimpl A A') -> ht_ded (ht A' c B') -> sat (eimpl B' B) ->
+    sat (eb_impl A A') -> ht_ded (ht A' c B') -> sat (eb_impl B' B) ->
     ht_ded (ht A c B)
-. 
+.
 
 Lemma ht_asgn_derived: forall (X : L) (a : AExp L) (A : EBExp L V),
     X ∉ aloc_vars a ∪ bloc_vars A ->
@@ -483,7 +524,7 @@ Context
   (Hin : i <> n)
   .
 
-Definition w : Cmd L := 
+Definition w : Cmd L :=
     While (ALe (Var i) (Var n))
       (Seq
       (Asgn s (Plus (Var s) (Var i)))
@@ -673,125 +714,5 @@ Proof.
       eapply IHHht; [done.. |].
       by eapply classical_satsi_impl; [apply H |].
 Qed.
-
-Section sec_weakest_precondition.
-
-Definition ws (c : Cmd L) (B : EBExp L V) (I : State V) : Ensemble (State L) :=
-    fun (sigma : State L) =>
-    forall (sigma' : State L), (sigma, sigma') ∈ denotc c -> satsi sigma' I B.
-
-Lemma ws_weakest :
-  forall (A B : EBExp L V) (c : Cmd L) (I : State V),
-  ht_sati I (ht A c B)
-    <->
-  sem I A ⊆ ws c B I.
-Proof. done. Qed.
-
-Section sec_wp_while.
-
-Context
-    (b : BExp L) (c : Cmd L) (w := While b c)
-    (B : EBExp L V).
-
-Inductive WhileOpenSequence : State L -> list (State L) -> State L -> Prop :=
-| ws_zero : forall (sigma : State L),
-    WhileOpenSequence sigma [sigma] sigma
-| ws_more : forall (sigma sigma' sigmaf : State L) (trace : list (State L)),
-    denotb b sigma = true ->
-    (sigma, sigma') ∈ denotc c ->
-    WhileOpenSequence sigma' trace sigmaf ->
-    WhileOpenSequence sigma (sigma :: trace) sigmaf
-.
-
-Lemma wos_first : forall (sigma sigma' : State L) (trace : list (State L)),
-    WhileOpenSequence sigma trace sigma' -> head trace = Some sigma.
-Proof. by intros *; inversion 1; subst. Qed.
-
-Lemma wos_last : forall (sigma sigma' : State L) (trace : list (State L)),
-    WhileOpenSequence sigma trace sigma' -> last trace = Some sigma'.
-Proof.
-    intros *; induction 1; [done |].
-    by rewrite last_cons, IHWhileOpenSequence.
-Qed.
-
-Record WhileSequence (sigma : State L) (trace : list (State L)) (sigma' : State L) : Prop :=
-{
-  ws_open : WhileOpenSequence sigma trace sigma';
-  ws_done : denotb b sigma' = false;
-}.
-
-Lemma ws_first : forall (sigma sigma' : State L) (trace : list (State L)),
-    WhileSequence sigma trace sigma' -> head trace = Some sigma.
-Proof. by intros * []; eapply wos_first. Qed.
-
-Lemma ws_last : forall (sigma sigma' : State L) (trace : list (State L)),
-    WhileSequence sigma trace sigma' -> last trace = Some sigma'.
-Proof. by intros * []; eapply wos_last. Qed.
-
-Lemma wp_claim1 :
-    forall  (sigma sigma' : State L),
-    (sigma, sigma') ∈ denotc w 
-      <->
-    exists (trace : list (State L)),
-    WhileSequence sigma trace sigma'.
-Proof.
-    intros; split.
-    - intro Hw.
-      pose (W (ss' : State L * State L) :=
-        exists (trace : list (State L)), WhileSequence ss'.1 trace ss'.2).
-      cut (denotc w ⊆ W);
-        [by intro Hincl; apply Hincl in Hw; apply Hw |].
-      apply knaster_tarski_least_pre_fixpoint.
-      clear.
-      intros (sigma, sigma').
-      unfold while_step; rewrite elem_of_relation_selector, elem_of_fwd_relation_composition.
-      intros [(Hb & sigma'' & Hc & trace & ? & ?) | [Hb Hdelta]].
-      + by exists (sigma :: trace); constructor; [econstructor |].
-      + inversion Hdelta; subst.
-        by exists [sigma']; constructor; [constructor |].
-    - intros [trace [Hw Hlst]].
-      induction Hw; (apply knaster_tarski_lfp_fix; [by typeclasses eauto |]).
-      + apply elem_of_relation_selector; right.
-        by split; [| constructor].
-      + apply elem_of_relation_selector; left.
-        split; [done |].
-        apply elem_of_fwd_relation_composition.
-        specialize (IHHw Hlst).
-        by eexists.
-Qed.
-
-Lemma wp_claim2 : forall (sigma : State L) (I : State V),
-    sigma ∈ ws w B I
-      <->
-    forall (sigma' : State L) (trace : list (State L)),
-        WhileOpenSequence sigma trace sigma' ->
-        satsi sigma' I (EOr b B).
-Proof.
-    intros. apply forall_proper; intros sigma'.
-    rewrite wp_claim1.
-    split; cycle 1.
-    - intros Hall (trace & Hw & Hlst).
-      specialize (Hall _ Hw).
-      apply satsi_or in Hall as [Hb |]; [| done].
-      by apply satsi_eval in Hb; rewrite Hb in Hlst.
-    - intros Hex trace Htrace.
-      rewrite satsi_or, satsi_eval.
-      destruct (denotb b sigma') eqn:Hb; [by left |].
-      right; apply Hex.
-      by exists trace; split.
-Qed.
-
-End sec_wp_while.
-
-Fixpoint wp (c : Cmd L) (B : EBExp L V) :=
-match c with
-| Skip => B
-| Asgn X a => bsubst B subst0 (mk_subst [(X, a)])
-| Seq c0 c1 => wp c0 (wp c1 B)
-| If b c0 c1 => EOr (EAnd b (wp c0 B)) (EAnd (ENot b) (wp c1 B))
-| _ => B
-end.
-
-End sec_weakest_precondition.
 
 End sec_axiomatic.
