theories/Semantics/IMP/AxiomaticCompleteness.v
@@ -1,0 +1,352 @@
+From stdpp Require Import prelude finite.
+From Coq Require Import Classical FunctionalExtensionality.
+From sets Require Import Functions Ensemble.
+
+From Semantics Require Import Syntax State Denotational Axiomatic GoedelBeta.
+
+
+Section sec_axiomatic_completeness.
+
+Context `{EqDecision L} `{EqDecision V}.
+
+Section sec_goedel.
+
+Context `{Infinite V}.
+
+Definition eb_mod (a b m : EAExp L V) (k := fresh (alog_vars a ∪ alog_vars b ∪ alog_vars m)): EBExp L V :=
+  EAnd (EAnd (EALe (EAVal 0)  a) (ENot (EALe b (EAVal 0))))
+  (eb_exists k (EAnd (EAnd (EAnd
+    (EALe (EAVal 0) (LVar k))
+    (EALe (EMul (LVar k) b) a)
+    ) (ENot (EALe (EMul (EPlus (LVar k) (EAVal 1)) b) a))
+    ) (EAEq m (EMinus a (EMul (LVar k) b))))).
+
+Lemma satsi_mod :
+    forall (a b m : EAExp L V) (sigma : State L) (I : State V),
+    satsi sigma I (eb_mod a b m)
+      <->
+    (eaeval sigma I a >= 0)%Z /\ (eaeval sigma I b > 0)%Z /\
+    ((eaeval sigma I a) mod (eaeval sigma I b))%Z = eaeval sigma I m.
+Proof.
+    intros.
+    unfold eb_mod.
+    rewrite !satsi_and, satsi_exists.
+    repeat setoid_rewrite satsi_and.
+    setoid_rewrite satsi_not.
+    repeat setoid_rewrite satsi_le.
+    repeat setoid_rewrite satsi_eq.
+    cbn; setoid_rewrite fn_update_eq.
+    remember (fresh _) as k.
+    assert (k ∉ alog_vars a ∪ alog_vars b ∪ alog_vars m)
+      by (subst k; apply is_fresh).
+    setoid_rewrite eaeval_update_I; [| by set_solver..].
+    clear.
+    generalize (eaeval sigma I a) as A; intro A.
+    generalize (eaeval sigma I b) as B; intro B.
+    generalize (eaeval sigma I m) as M; intro M.
+    unfold Z.modulo.
+    destruct Z.div_eucl as (d', m') eqn: Hdm.
+    pose (Hdiv_mod := Z_div_mod_full A B); rewrite Hdm in Hdiv_mod; clear Hdm.
+    split.
+    - intros ([Ha Hb] & d & [[Hd0 Hd1] Hd2] & Hdm).
+      split; [by lia |].
+      split; [by lia |].
+      destruct Hdiv_mod as [-> [Hrem | Hrem]]; [by lia | | by lia].
+      cut (d = d'); [by lia |]; clear Hdm.
+      assert (d - d' < 1)%Z by nia.
+      assert (d - d' > -1)%Z by nia.
+      by lia.
+    - intros (Ha & Hb & <-).
+      destruct Hdiv_mod as [-> [Hrem | Hrem]]; [by lia | | by lia].
+      split; [by lia |].
+      exists d'.
+      split; [by nia | by lia].
+Qed.
+
+Definition eb_beta (a b i x : EAExp L V) : EBExp L V :=
+    EAnd (EAnd (EALe (EAVal 0) b) (EALe (EAVal 0) i))
+    (eb_mod a (EPlus (EAVal 1) (EMul (EPlus (EAVal 1) i) b)) x).
+
+Lemma satsi_beta : forall (a b i x : EAExp L V) (sigma : State L) (I : State V),
+    satsi sigma I (eb_beta a b i x)
+      <->
+    (eaeval sigma I a >=0)%Z /\
+    (eaeval sigma I b >=0)%Z /\
+    (eaeval sigma I i >=0)%Z /\
+    eaeval sigma I x
+      =
+    Z.of_nat (beta_fn (Z.to_nat (eaeval sigma I a)) (Z.to_nat (eaeval sigma I b)) (Z.to_nat (eaeval sigma I i))).
+Proof.
+    intros.
+    unfold eb_beta, beta_fn; rewrite !satsi_and, satsi_mod, !satsi_le; cbn.
+    generalize (eaeval sigma I a) as A; intro A.
+    generalize (eaeval sigma I b) as B; intro B.
+    generalize (eaeval sigma I i) as J; intro J.
+    generalize (eaeval sigma I x) as X; intro X.
+    destruct PeanoNat.Nat.divmod as (q, r) eqn:Hdm.
+    specialize
+      (PeanoNat.Nat.divmod_spec
+        (Z.to_nat A) (Z.to_nat B + Z.to_nat J * Z.to_nat B)
+        0 (Z.to_nat B + Z.to_nat J * Z.to_nat B)).
+    rewrite Hdm; clear Hdm.
+    intros [Hdm Hr]; [done |].
+    unfold Z.modulo.
+    destruct Z.div_eucl as (d', m') eqn: Hdm'.
+    pose (Hdiv_mod := Z_div_mod_full A (1 + (1 + J) * B)); rewrite Hdm' in Hdiv_mod; clear Hdm'.
+    split.
+    - intros ([Hb Hj] & Ha & Hd & <-).
+      split; [by lia |].
+      split; [by lia |].
+      split; [by lia |].
+      destruct Hdiv_mod as [-> [Hm' | Hm']]; [by lia | | by lia].
+      cbn.
+      clear a b i x.
+      assert
+          (Hdm' : ((1 + B + J * B) * (d' - Z.of_nat q))%Z
+            =
+           (B + J *  B - Z.of_nat r - m')%Z)
+          by lia.
+      clear Hdm.
+      cut (d' = Z.of_nat q); [by lia |].
+      assert (Hd' : (1 + B + J * B > 0)%Z) by nia.
+      assert (Hrm' : (- (1 + B + J * B) < (B + J *  B - Z.of_nat r - m') < 1 + B + J * B)%Z) by lia.
+      clear Hm' Hd.
+      assert (Hqd'lt' : ((1 + B + J * B) * (d' - Z.of_nat q - 1) < 0)%Z ) by lia.
+      assert (Hqs'gt' : ((1 + B + J * B) * ((d' - Z.of_nat q) + 1) > 0)%Z ) by lia.
+      apply Z.lt_mul_0 in Hqd'lt' as [|[_ Hqd'lt'']]; [by lia |].
+      apply Zmult_gt_0_reg_l in Hqs'gt'; [| done].
+      by lia.
+    - intros (Ha & Hb & Hj & ->).
+      split_and!; [by lia.. |].
+      assert
+          (Hdm' : ((1 + B + J * B) * (d' - Z.of_nat q))%Z
+            =
+           (B + J *  B - Z.of_nat r - m')%Z)
+          by lia.
+      clear Hdm.
+      destruct Hdiv_mod as [-> [Hm' | Hm']]; [by lia | | by lia].
+      cbn.
+      cut (d' = Z.of_nat q); [by lia |].
+      assert (Hd' : (1 + B + J * B > 0)%Z) by nia.
+      assert (Hrm' : (- (1 + B + J * B) < (B + J *  B - Z.of_nat r - m') < 1 + B + J * B)%Z) by lia.
+      assert (Hqd'lt' : ((1 + B + J * B) * (d' - Z.of_nat q - 1) < 0)%Z ) by lia.
+      assert (Hqs'gt' : ((1 + B + J * B) * ((d' - Z.of_nat q) + 1) > 0)%Z ) by lia.
+      apply Z.lt_mul_0 in Hqd'lt' as [|[_ Hqd'lt'']]; [by lia |].
+      apply Zmult_gt_0_reg_l in Hqs'gt'; [| done].
+      by lia.
+Qed.
+
+Definition beta_z_helper (x : nat) (y : Z) : Prop :=
+    exists (z : nat),
+      (x = 2 * z -> y = Z.of_nat z)
+        /\
+      (x = 2 * z + 1 -> y = (- Z.of_nat z)%Z).
+
+Definition eb_beta_z_helper (x y : EAExp L V) (z := fresh (alog_vars x ∪ alog_vars y)) : EBExp L V :=
+    EAnd (EALe (EAVal 0) x)
+    (eb_exists z
+        (EAnd (EALe (EAVal 0) (LVar z))
+         (EAnd (eb_impl (EAEq x (EMul (EAVal 2) (LVar z))) (EAEq y (LVar z)))
+               (eb_impl (EAEq x (EPlus (EMul (EAVal 2) (LVar z)) (EAVal 1))) (EAEq y (EMinus (EAVal 0) (LVar z))))))).
+
+Lemma satsi_beta_z_helper: forall (x y : EAExp L V) (sigma : State L) (I : State V),
+    satsi sigma I (eb_beta_z_helper x y)
+      <->
+    (eaeval sigma I x >= 0)%Z
+      /\
+    beta_z_helper (Z.to_nat (eaeval sigma I x)) (eaeval sigma I y).
+Proof.
+    intros; unfold eb_beta_z_helper, beta_z_helper.
+    rewrite satsi_and, satsi_exists.
+    do 2 setoid_rewrite satsi_and.
+    setoid_rewrite classical_satsi_impl.
+    setoid_rewrite satsi_eq.
+    setoid_rewrite satsi_le.
+    cbn.
+    setoid_rewrite fn_update_eq.
+    remember (fresh _) as k.
+    assert (Hk: k ∉ alog_vars x ∪ alog_vars y)
+      by (subst k; apply is_fresh).
+    setoid_rewrite eaeval_update_I; [| by set_solver..].
+    clear k Heqk Hk.
+    generalize (eaeval sigma I x) as X; intro X.
+    generalize (eaeval sigma I y) as Y; intro Y.
+    split.
+    - intros (HX & z & Hz & Heven & Hodd).
+      split; [by lia |].
+      by exists (Z.to_nat z); split; lia.
+    - intros (HX & z & Heven & Hodd).
+      split; [by lia |].
+      by exists (Z.of_nat z); lia.
+Qed.
+
+Definition beta_z (n m j : nat) (y : Z) : Prop :=
+    beta_z_helper (beta_fn n m j) y.
+
+Definition eb_beta_z (n m j y : EAExp L V)
+    (x := fresh (alog_vars n ∪ alog_vars m ∪ alog_vars j ∪ alog_vars y)) : EBExp L V :=
+    eb_exists x
+        (EAnd (eb_beta n m j (LVar x)) (eb_beta_z_helper (LVar x) y)).
+
+Lemma satsi_beta_z : forall (n m j y : EAExp L V) (sigma : State L) (I : State V),
+    satsi sigma I (eb_beta_z n m j y)
+      <->
+    (eaeval sigma I n >= 0)%Z
+      /\
+    (eaeval sigma I m >= 0)%Z
+      /\
+    (eaeval sigma I j >= 0)%Z
+      /\
+    beta_z (Z.to_nat (eaeval sigma I n)) (Z.to_nat (eaeval sigma I m)) (Z.to_nat (eaeval sigma I j)) (eaeval sigma I y).
+Proof.
+    intros; unfold eb_beta_z, beta_z.
+    rewrite satsi_exists.
+    setoid_rewrite satsi_and.
+    setoid_rewrite satsi_beta.
+    setoid_rewrite satsi_beta_z_helper.
+    setoid_rewrite fn_update_eq.
+    remember (fresh _) as k.
+    assert (Hk: k ∉ alog_vars n ∪ alog_vars m ∪ alog_vars j ∪ alog_vars y)
+      by (subst k; apply is_fresh).
+    setoid_rewrite eaeval_update_I; [| by set_solver..].
+    clear k Heqk Hk.
+    generalize (eaeval sigma I n); intro N.
+    generalize (eaeval sigma I m); intro M.
+    generalize (eaeval sigma I j); intro J.
+    generalize (eaeval sigma I y); intro Y.
+    generalize (beta_fn (Z.to_nat N) (Z.to_nat M) (Z.to_nat J)); intro B.
+    split.
+    - intros (z & (Hn & Hm & Hj & ->) & Hz & Hbeta).
+      by rewrite Nat2Z.id in Hbeta.
+    - intros (Hn & Hm & Hj & Hbeta).
+      exists (Z.of_nat B).
+      rewrite Nat2Z.id.
+      by split_and!; [..| lia |].
+Qed.
+
+End sec_goedel.
+
+(*
+Section sec_weakest_precondition.
+
+Definition ws (c : Cmd L) (B : EBExp L V) (I : State V) : Ensemble (State L) :=
+    fun (sigma : State L) =>
+    forall (sigma' : State L), (sigma, sigma') ∈ denotc c -> satsi sigma' I B.
+
+Lemma ws_weakest :
+  forall (A B : EBExp L V) (c : Cmd L) (I : State V),
+  ht_sati I (ht A c B)
+    <->
+  sem I A ⊆ ws c B I.
+Proof. done. Qed.
+
+Section sec_wp_while.
+
+Context
+    (b : BExp L) (c : Cmd L) (w : Cmd L := While b c)
+    (B : EBExp L V)
+    (relevant_vars : list L := elements (bloc_vars B ∪ cloc_vars w))
+    .
+
+Inductive WhileOpenSequence : State L -> list (State L) -> State L -> Prop :=
+| ws_zero : forall (sigma : State L),
+    WhileOpenSequence sigma [sigma] sigma
+| ws_more : forall (sigma sigma' sigmaf : State L) (trace : list (State L)),
+    denotb b sigma = true ->
+    (sigma, sigma') ∈ denotc c ->
+    WhileOpenSequence sigma' trace sigmaf ->
+    WhileOpenSequence sigma (sigma :: trace) sigmaf
+.
+
+Lemma wos_first : forall (sigma sigma' : State L) (trace : list (State L)),
+    WhileOpenSequence sigma trace sigma' -> head trace = Some sigma.
+Proof. by intros *; inversion 1; subst. Qed.
+
+Lemma wos_last : forall (sigma sigma' : State L) (trace : list (State L)),
+    WhileOpenSequence sigma trace sigma' -> last trace = Some sigma'.
+Proof.
+    intros *; induction 1; [done |].
+    by rewrite last_cons, IHWhileOpenSequence.
+Qed.
+
+Record WhileSequence (sigma : State L) (trace : list (State L)) (sigma' : State L) : Prop :=
+{
+  ws_open : WhileOpenSequence sigma trace sigma';
+  ws_done : denotb b sigma' = false;
+}.
+
+Lemma ws_first : forall (sigma sigma' : State L) (trace : list (State L)),
+    WhileSequence sigma trace sigma' -> head trace = Some sigma.
+Proof. by intros * []; eapply wos_first. Qed.
+
+Lemma ws_last : forall (sigma sigma' : State L) (trace : list (State L)),
+    WhileSequence sigma trace sigma' -> last trace = Some sigma'.
+Proof. by intros * []; eapply wos_last. Qed.
+
+Lemma wp_claim1 :
+    forall  (sigma sigma' : State L),
+    (sigma, sigma') ∈ denotc w
+      <->
+    exists (trace : list (State L)),
+    WhileSequence sigma trace sigma'.
+Proof.
+    intros; split.
+    - intro Hw.
+      pose (W (ss' : State L * State L) :=
+        exists (trace : list (State L)), WhileSequence ss'.1 trace ss'.2).
+      cut (denotc w ⊆ W);
+        [by intro Hincl; apply Hincl in Hw; apply Hw |].
+      apply knaster_tarski_least_pre_fixpoint.
+      clear.
+      intros (sigma, sigma').
+      unfold while_step; rewrite elem_of_relation_selector, elem_of_fwd_relation_composition.
+      intros [(Hb & sigma'' & Hc & trace & ? & ?) | [Hb Hdelta]].
+      + by exists (sigma :: trace); constructor; [econstructor |].
+      + inversion Hdelta; subst.
+        by exists [sigma']; constructor; [constructor |].
+    - intros [trace [Hw Hlst]].
+      induction Hw; (apply knaster_tarski_lfp_fix; [by typeclasses eauto |]).
+      + apply elem_of_relation_selector; right.
+        by split; [| constructor].
+      + apply elem_of_relation_selector; left.
+        split; [done |].
+        apply elem_of_fwd_relation_composition.
+        specialize (IHHw Hlst).
+        by eexists.
+Qed.
+
+Lemma wp_claim2 : forall (sigma : State L) (I : State V),
+    sigma ∈ ws w B I
+      <->
+    forall (sigma' : State L) (trace : list (State L)),
+        WhileOpenSequence sigma trace sigma' ->
+        satsi sigma' I (EOr b B).
+Proof.
+    intros. apply forall_proper; intros sigma'.
+    rewrite wp_claim1.
+    split; cycle 1.
+    - intros Hall (trace & Hw & Hlst).
+      specialize (Hall _ Hw).
+      apply satsi_or in Hall as [Hb |]; [| done].
+      by apply satsi_eval in Hb; rewrite Hb in Hlst.
+    - intros Hex trace Htrace.
+      rewrite satsi_or, satsi_eval.
+      destruct (denotb b sigma') eqn:Hb; [by left |].
+      right; apply Hex.
+      by exists trace; split.
+Qed.
+
+End sec_wp_while.
+
+Fixpoint wp (c : Cmd L) (B : EBExp L V) :=
+match c with
+| Skip => B
+| Asgn X a => bsubst B subst0 (mk_subst [(X, a)])
+| Seq c0 c1 => wp c0 (wp c1 B)
+| If b c0 c1 => EOr (EAnd b (wp c0 B)) (EAnd (ENot b) (wp c1 B))
+| _ => B
+end.
+
+End sec_weakest_precondition.
+*)
+End sec_axiomatic_completeness.
