theories/Semantics/IMP/GoedelBeta.v
@@ -1,0 +1,378 @@
+From stdpp Require Import prelude finite.
+From Coq Require Import IndefiniteDescription.
+
+Definition beta_fn (a b i : nat) : nat := a `mod` (1 + (1 + i) * b).
+
+Definition beta_p (m : nat) `(i : fin k) : nat := 1 + (1 + (fin_to_nat i)) * m.
+
+Definition beta_m `(a : fin k -> nat) :=
+  fact (max k (max_list (map a (enum (fin k))))).
+
+Definition beta_pa `(a : fin k -> nat) (i : fin k) : nat :=
+  beta_p (beta_m a) i.
+
+Lemma fact_ge_n : forall (n : nat), n <= fact n.
+Proof.
+    induction n; cbn; [by lia |].
+    by cut (0 < fact n); [nia | apply lt_O_fact].
+Qed.
+
+Lemma fact_ge_1 : forall (n : nat), 1 <= fact n.
+Proof.
+    induction n; cbn; [by lia |].
+    by cut (0 < fact n); [nia | apply lt_O_fact].
+Qed.
+
+Lemma beta_lemma_a1 :
+    forall (k : nat) (a : fin k -> nat),
+    forall (i : fin k), a i < beta_pa a i.
+Proof.
+    intros.
+    pose (max_a := max_list (map a (enum (fin k)))).
+    pose (m := fact (max k max_a)).
+    assert (Hai : a i <= k `max` max_a).
+    {
+      cut (a i <= max_a); [by lia |].
+      apply max_list_elem_of_le, elem_of_list_fmap.
+      by eexists; split; [| apply elem_of_enum].
+    }
+    unfold beta_p.
+    remember (k `max` max_a) as maxx.
+    subst m max_a; unfold beta_pa, beta_p, beta_m.
+    rewrite <- Heqmaxx.
+    specialize (fact_ge_n maxx).
+    by lia.
+Qed.
+
+Lemma beta_lemma_a2:
+    forall (k : nat) (a : fin k -> nat),
+    forall (i j : fin k), j < i -> Nat.gcd (beta_pa a i) (beta_pa a j) = 1.
+Proof.
+    intros.
+    pose (max_a := max_list (map a (enum (fin k)))).
+    pose (m := fact (max k max_a)).
+    unfold beta_p.
+    remember (Nat.gcd _ _) as d.
+    assert (Hdi : (d | beta_p m i)) by (subst; apply Nat.gcd_divide_l).
+    assert (Hdj : (d | beta_p m j)) by (subst; apply Nat.gcd_divide_r).
+    assert (Hdijm : (d | beta_p m i - beta_p m j)) by (apply Nat.divide_sub_r; done).
+    replace (beta_p m i - beta_p m j) with ((i - j) * m) in Hdijm
+      by (unfold beta_p; nia).
+    apply Nat.divide_mul_l with (p := (i - j)) in Hdi as Hdi'.
+    apply Nat.divide_mul_l with (p := (1 + i)) in Hdijm as Hdijm'.
+    assert (Hdij : (d | beta_p m i * (i - j) - (i - j) * m * (1 + i)))
+       by (apply Nat.divide_sub_r; done).
+    replace (beta_p m i * (i - j) - (i - j) * m * (1 + i)) with (i - j) in Hdij
+      by (unfold beta_p; nia).
+    assert (i - j | m) as [mij ->].
+    {
+      subst m.
+      cut (forall (m n : nat), 0 < m <= n -> (m | fact n)).
+      {
+        intro Hdiv; apply Hdiv; split; [by lia |].
+        etransitivity; [| by apply Nat.le_max_l].
+        etransitivity; [by apply Nat.le_sub_l |].
+        by specialize (fin_to_nat_lt i); lia.
+      }
+      intros m n; revert m; induction n; [by lia |].
+      intros m Hm. change (fact (S n)) with (S n * fact n).
+      destruct (decide (m = S n));
+        [by subst; apply Nat.divide_mul_l |].
+      by apply Nat.divide_mul_r, IHn; lia.
+    }
+    apply Nat.divide_mul_l with (p := (1 + i) * mij) in Hdij as Hdij'.
+    assert (Hdone : (d | beta_p (mij * (i - j)) i - (i - j) * ((1 + i) * mij)))
+      by (apply Nat.divide_sub_r; done).
+    replace ((beta_p (mij * (i - j)) i - (i - j) * ((1 + i) * mij))) with 1
+      in Hdone by (unfold beta_p; nia).
+    by apply Nat.divide_1_r.
+Qed.
+
+Definition prod_list_with {A} (f : A → nat) : list A → nat :=
+    fix go l :=
+    match l with
+    | [] => 1
+    | x :: l => f x * go l
+    end.
+
+Lemma prod_list_with_cons : forall `(f : A -> nat) (a : A) (l : list A),
+    prod_list_with f (a :: l) = f a * prod_list_with f l.
+Proof. done. Qed.
+
+Lemma prod_list_with_not_zero : forall `(f : A -> nat) (l : list A),
+    List.Forall (fun x => f x <> 0) l -> prod_list_with f l <> 0.
+Proof. by intros *; induction 1; cbn; [| lia]. Qed.
+
+Lemma prod_list_with_filter :
+    forall `(f : A → nat) (P : A -> Prop) `{forall a, Decision (P a)} (l : list A),
+    prod_list_with f l = prod_list_with f (filter P l) * prod_list_with f (filter (not ∘ P) l).
+Proof.
+    induction l; [done |].
+    cbn.
+    case_decide.
+    - rewrite decide_False by (intro; done).
+      by cbn; rewrite IHl, Nat.mul_assoc.
+    - rewrite decide_True by done.
+      cbn; rewrite IHl, !Nat.mul_assoc.
+      by f_equal; apply Nat.mul_comm.
+Qed.
+
+Lemma sum_list_with_filter :
+    forall `(f : A → nat) (P : A -> Prop) `{forall a, Decision (P a)} (l : list A),
+    sum_list_with f l = sum_list_with f (filter P l) + sum_list_with f (filter (not ∘ P) l).
+Proof.
+    induction l; [done |].
+    cbn.
+    case_decide.
+    - rewrite decide_False by (intro; done).
+      by cbn; rewrite IHl, Nat.add_assoc.
+    - rewrite decide_True by done.
+      cbn; rewrite IHl, !Nat.add_assoc.
+      by f_equal; apply Nat.add_comm.
+Qed.
+
+Lemma sum_list_with_mod : forall `(f : A -> nat) (l : list A) (n : nat),
+    sum_list_with f l `mod` n = sum_list_with (fun a => f a `mod` n) l `mod` n.
+Proof.
+    intros; induction l; cbn; [done |].
+    by rewrite Nat.Div0.add_mod, IHl, Nat.Div0.add_mod_idemp_r.
+Qed.
+
+Lemma sum_list_with_0 :  forall `(f : A -> nat) (l : list A),
+    List.Forall (fun a => f a = 0) l ->
+    sum_list_with f l = 0.
+Proof. by intros *; induction 1; cbn; [| lia]. Qed.
+
+Lemma gcd_1_mul : forall (n fl fa : nat), n <> 0 ->
+    Nat.gcd fl n = 1 -> Nat.gcd fa n = 1 -> Nat.gcd (fa * fl) n = 1.
+Proof.
+    intros * Hn Hfl Hfa.
+    destruct n; [done |].
+    destruct n.
+    - destruct (decide (fa * fl = 0)); [by rewrite e; apply Nat.gcd_0_l |].
+      apply Nat.bezout_1_gcd; unfold Nat.Bezout.
+      by exists 1, (fa * fl - 1); nia.
+    - destruct (Nat.gcd_bezout_pos (S (S n)) fa) as (xa & ya & Hxya); [lia |].
+      rewrite Nat.gcd_comm, Hfa in Hxya; clear Hfa.
+      destruct (Nat.gcd_bezout_pos (S (S n)) fl) as (xl & yl & Hxyl); [lia |].
+      rewrite Nat.gcd_comm, Hfl in Hxyl; clear Hfl.
+      apply Nat.bezout_1_gcd; unfold Nat.Bezout.
+      exists (ya * yl),  (xa * xl * S (S n) - xa - xl).
+      replace ((xa * xl * S (S n) - xa - xl) * S (S n)) with
+        ((xa * S (S n)) * (xl * S (S n)) - xa * S (S n) - xl * S (S n)) by nia.
+      rewrite !Hxya, !Hxyl.
+      assert (ya * fa <> 0) by (intro Hrew; rewrite Hrew in Hxya; lia).
+      assert (yl * fl <> 0) by (intro Hrew; rewrite Hrew in Hxyl; lia).
+      assert (ya * yl * (fa * fl) <> 0) by nia.
+      replace ((1 + ya * fa) * (1 + yl * fl)) with (ya * yl * (fa * fl) + (1 + ya * fa) + yl * fl) by nia.
+      by lia.
+Qed.
+
+Lemma prod_list_with_gcd :
+    forall `(f : A -> nat) (l : list A) (n : nat), n <> 0 ->
+    List.Forall (fun i => Nat.gcd (f i) n = 1) l ->
+    Nat.gcd (prod_list_with f l) n = 1.
+Proof.
+    intros * Hn; induction l;
+      [by intros _; apply Nat.bezout_1_gcd; exists 1, 0 |].
+    rewrite Forall_cons; intros [Ha Hall].
+    specialize (IHl Hall); clear Hall.
+    rewrite prod_list_with_cons.
+    by apply gcd_1_mul.
+Qed.
+
+Lemma prod_list_with_in : forall (A : Type) (x : A) (f : A → nat) (ls : list A),
+    x ∈ ls -> (f x | prod_list_with f ls).
+Proof.
+    induction 1; [by cbn; rewrite Nat.mul_comm; eexists |].
+    destruct IHelem_of_list as [a Ha].
+    cbn; rewrite Ha.
+    by exists (f y * a); nia.
+Qed.
+
+Definition beta_pa_product `(a : fin k -> nat) : nat :=
+    prod_list_with (beta_pa a) (enum (fin k)).
+
+Definition beta_c `(a : fin k -> nat) (i : fin k) : nat :=
+    prod_list_with (beta_pa a) (filter (fun j => j <> i) (enum (fin k))).
+
+Lemma filter_singleton : forall (A : Type) `{EqDecision A} (l : list A) (a : A),
+  NoDup l -> a ∈ l -> filter (fun b => b = a) l = [a].
+Proof.
+    intros * Hnodup Ha.
+    apply Permutation_singleton_r, NoDup_Permutation_bis.
+    - by apply NoDup_ListNoDup, NoDup_filter.
+    - cut ( length (filter (λ b : A, b = a) l)
+            =
+            if decide(a ∈ l) then 1 else 0);
+        [by intros ->; rewrite decide_True |].
+      revert Hnodup; clear; induction l; cbn;
+        [by rewrite decide_False; [| inversion 1] |].
+      rewrite NoDup_cons; intros [Ha0 Hnodup].
+      destruct (decide (a0 = a)).
+      + subst; rewrite decide_True by left.
+        rewrite decide_False in IHl by done; cbn.
+        by unfold filter in *; cbn in *; rewrite IHl.
+      + unfold filter in *; cbn in *; rewrite IHl by done.
+        case_decide.
+        * by rewrite decide_True by (right; done).
+        * by rewrite decide_False; [| inversion 1].
+    - intros j. rewrite <- !elem_of_list_In, elem_of_list_singleton, elem_of_list_filter.
+      by intros [-> _].
+Qed.
+
+Lemma beta_c_char : forall `(a : fin k -> nat) (i : fin k),
+    beta_pa_product a = beta_c a i * beta_pa a i.
+Proof.
+    intros.
+    unfold beta_pa_product.
+    erewrite prod_list_with_filter with (P := fun j => j <> i).
+    f_equal.
+    erewrite list_filter_iff with (P2 := fun j => j = i), filter_singleton.
+    - by cbn; lia.
+    - by apply NoDup_enum.
+    - by apply elem_of_enum.
+    - intro; cbn; split; intro Hxi.
+      + by destruct (decide (x = i)).
+      + by destruct (decide (x <> i)).
+Qed.
+
+Lemma Zn_multiplicative_inverse :
+    forall (m n : nat), m <> 0 -> 1 < n -> Nat.gcd m n = 1 ->
+    exists! (d : nat), d < n /\ (d * m) `mod` n = 1.
+Proof.
+    intros * Hm Hn Hgcd.
+    destruct (Nat.gcd_bezout_pos m n) as (a & b & Hab); [by lia |].
+    rewrite Hgcd in Hab.
+    assert (Hmod : (a `mod` n * m) `mod` n = 1).
+    {
+      rewrite Nat.Div0.mul_mod_idemp_l, Hab.
+      rewrite Nat.Div0.mod_add.
+      by apply Nat.mod_1_l; lia.
+    }
+    exists (a `mod` n); split.
+    - split; [| done].
+      by apply Nat.mod_bound_pos; lia.
+    - intros a' [Ha' Hmod'].
+      rewrite Nat.Div0.mod_eq in Hmod', Hmod at 1.
+      destruct (decide (a' <= a `mod` n)).
+      + assert (Hdiv: (n | a `mod` n - a')).
+        {
+          apply Nat.gauss with m; [| by rewrite Nat.gcd_comm].
+          exists ((a `mod` n * m) `div` n - (a' * m) `div` n).
+          by nia.
+        }
+        assert (a `mod` n - a' < n).
+        {
+          cut (a `mod` n < n); [by lia |].
+          by apply Nat.mod_upper_bound; lia.
+        }
+        destruct (decide (a `mod` n - a' = 0)); [by lia |].
+        apply Nat.divide_pos_le in Hdiv; by lia.
+      + assert (Hdiv: (n | a' - a `mod` n)).
+        {
+          apply Nat.gauss with m; [| by rewrite Nat.gcd_comm].
+          exists ((a' * m) `div` n - (a `mod` n * m) `div` n).
+          by nia.
+        }
+        assert (a' - a `mod` n < n).
+        {
+          cut (a `mod` n < n); [by lia |].
+          by apply Nat.mod_upper_bound; lia.
+        }
+        destruct (decide (a' - a `mod` n = 0)); [by lia |].
+        apply Nat.divide_pos_le in Hdiv; by lia.
+Qed.
+
+Lemma beta_lemma_b :
+    forall (k : nat) (a : fin k -> nat) (i : fin k),
+    exists! (d : nat), d < beta_pa a i /\ (d * beta_c a i) `mod` beta_pa a i = 1.
+Proof.
+    intros.
+    apply Zn_multiplicative_inverse.
+    - apply prod_list_with_not_zero.
+      apply Forall_forall; intros j _.
+      by unfold beta_pa, beta_p; lia.
+    - unfold beta_pa, beta_p, beta_m.
+      by specialize (fact_ge_1 (k `max` max_list (map a (enum (fin k))))); nia.
+    - apply prod_list_with_gcd.
+      + by unfold beta_pa, beta_p; lia.
+      + apply Forall_forall; intro j.
+        rewrite elem_of_list_filter; intros [Hij _].
+        destruct (decide (i < j)); [by apply beta_lemma_a2 |].
+        rewrite Nat.gcd_comm; apply beta_lemma_a2.
+        cut (fin_to_nat i <> fin_to_nat j); [by lia |].
+        clear -Hij.
+        contradict Hij.
+        pose proof (Hi := fin_to_nat_lt i).
+        rewrite <- nat_to_fin_to_nat with (H := Hi).
+        revert Hi.
+        rewrite Hij.
+        intro Hj.
+        by rewrite nat_to_fin_to_nat.
+Qed.
+
+Definition beta_lemma_b_choice `(a : fin k -> nat) (i : fin k) :
+    {d : nat | d < beta_pa a i /\ (d * beta_c a i) `mod` beta_pa a i = 1}.
+Proof.
+    apply constructive_definite_description, beta_lemma_b.
+Qed.
+
+Definition beta_d `(a : fin k -> nat) (i : fin k) : nat :=
+    proj1_sig (beta_lemma_b_choice a i).
+
+Lemma beta_d_prop1 : forall (k : nat) (a : fin k -> nat) (i : fin k),
+    beta_d a i < beta_pa a i.
+Proof.
+    intros. unfold beta_d.
+    by destruct beta_lemma_b_choice as (? & ? & ?).
+Qed.
+
+Lemma beta_d_prop2 : forall (k : nat) (a : fin k -> nat) (i : fin k),
+    (beta_c a i * beta_d a i) `mod` beta_pa a i = 1.
+Proof.
+    intros. rewrite Nat.mul_comm. unfold beta_d.
+    by destruct beta_lemma_b_choice as (? & ? & ?).
+Qed.
+
+Definition beta_n `(a : fin k -> nat) :=
+    sum_list_with (fun i => beta_c a i * beta_d a i * a i) (enum (fin k)).
+
+Lemma beta_lemma_c : forall (k : nat) (a : fin k -> nat) (i : fin k),
+    beta_n a `mod` beta_pa a i = a i.
+Proof.
+    intros.
+    unfold beta_n.
+    erewrite sum_list_with_filter with (P := fun j => j = i), filter_singleton;
+      [| by apply NoDup_enum | by apply elem_of_enum].
+    replace (sum_list_with (λ i0 : fin k, beta_c a i0 * beta_d a i0 * a i0) [i])
+      with (beta_c a i * beta_d a i * a i)
+      by (cbn; lia).
+    rewrite Nat.Div0.add_mod.
+    replace (sum_list_with _ _ `mod` beta_pa a i) with 0.
+    - replace ((beta_c a i * beta_d a i * a i) `mod` beta_pa a i) with (a i).
+      + replace (a i + 0) with (a i) by lia.
+        by apply Nat.mod_small, beta_lemma_a1.
+      + rewrite <- Nat.Div0.mul_mod_idemp_l, beta_d_prop2.
+        replace (1 * a i) with (a i) by lia.
+        by symmetry; apply Nat.mod_small, beta_lemma_a1.
+    - rewrite sum_list_with_mod, sum_list_with_0, Nat.Div0.mod_0_l; [done |].
+      apply Forall_forall; intro j.
+      rewrite elem_of_list_filter; intros [Hj _]; cbn in Hj.
+      rewrite <- Nat.mul_assoc, <- Nat.Div0.mul_mod_idemp_l.
+      replace (beta_c a j `mod` beta_pa a i) with 0; [by apply Nat.Div0.mod_0_l |].
+      symmetry; apply Nat.Lcm0.mod_divide.
+      apply prod_list_with_in, elem_of_list_filter.
+      by split; [| apply elem_of_enum].
+Qed.
+
+Lemma beta_lemma :
+    forall (k : nat) (a : fin k -> nat),
+    exists (n m : nat),
+        forall (j : fin k),
+        beta_fn n m j = a j.
+Proof.
+    intros.
+    exists (beta_n a), (beta_m a).
+    by apply beta_lemma_c.
+Qed.
